Setlec/Model/Annotate.lean
@@ -348,18 +348,13 @@ theorem annotateCore_sound (m : EnvModel V env) :
       annotateCore_sound m fuel e he hw hb hLbe ρ hoke
     rcases hres with ⟨us, A, B, cv, caps, hteq, hfind, hi2, rfl⟩ | hel
     case inr =>
-      obtain ⟨us, pcv, nP, nM, nm, ni, rules, -, -, -,
-        hwsb, hrb, hall, hann⟩ := annotateProjElim_inv hel
-      have hsubR : ∀ l ∈ (Expr.mkAppN (.const (projFnName sn i) us)
-          (te'.getAppArgs ++ [e₂])).fvarLeaves,
-          l ∈ e₂.fvarLeaves := fun l hl => by
+      obtain ⟨raw, hwsb, hrb, hall, hann⟩ := annotateProjElim_inv hel
+      have hsubR : ∀ l ∈ raw.fvarLeaves, l ∈ e₂.fvarLeaves := fun l hl => by
         have := List.all_eq_true.mp hall l hl
         simpa using this
-      have hLbraw : Expr.LeavesBounded (Expr.mkAppN
-          (.const (projFnName sn i) us) (te'.getAppArgs ++ [e₂])) :=
+      have hLbraw : Expr.LeavesBounded raw :=
         fun l hl => hLbe l (hsl l (hsubR l hl))
-      have hokraw : FvarsOk V m.val env φ d ρ (Expr.mkAppN
-          (.const (projFnName sn i) us) (te'.getAppArgs ++ [e₂])) :=
+      have hokraw : FvarsOk V m.val env φ d ρ raw :=
         fun l hl => hoke l (hsl l (hsubR l hl))
       exact annotateCore_sound m fuel _ hann (WScoped.of_wscopedB hwsb)
         hrb hLbraw ρ hokraw
